theories/Basics/Notations.v
@@ -37,6 +37,7 @@ Reserved Notation "F '_0' x" (at level 10, no associativity).
 Reserved Notation "F '_0' x" (at level 10, no associativity, only parsing).
 Reserved Notation "f ^-1" (at level 3, format "f '^-1'").
 Reserved Notation "f ^-1*" (at level 3, format "f '^-1*'").
+Reserved Notation "f ^-1$" (at level 3, format "f '^-1$'").
 Reserved Notation "F '_1' m" (at level 10, no associativity).
 Reserved Notation "f ^*" (at level 20).
 Reserved Notation "f ^$" (at level 20).
